Tidy up

experiments/Tree_Traversal.thy
@@ -16,69 +16,49 @@ where
     "labels (Leaf x) = [x]"
   | "labels (Node l r) = labels l @ labels r"
 
-definition [applicative_unfold]: "liftSt1 f x = Pair f \<diamond> x"
-definition [applicative_unfold]: "liftSt2 f x y = Pair f \<diamond> x \<diamond> y"
+definition fresh :: "(nat, nat) state"
+where "fresh n = (n, n + 1)"
 
-definition "fresh n = (n, n + 1)"
-
-primrec number_tree :: "'a tree \<Rightarrow> nat \<Rightarrow> nat tree \<times> nat"
+primrec number_tree :: "'a tree \<Rightarrow> (nat tree, nat) state"
 where
-    "number_tree (Leaf _) = liftSt1 Leaf fresh"
-  | "number_tree (Node l r) = liftSt2 Node (number_tree l) (number_tree r)"
+    "number_tree (Leaf _) = pure_state Leaf \<diamond> fresh"
+  | "number_tree (Node l r) = pure_state Node \<diamond> number_tree l \<diamond> number_tree r"
 
-primrec number_list :: "'a list \<Rightarrow> nat \<Rightarrow> nat list \<times> nat"
+primrec number_list :: "'a list \<Rightarrow> (nat list, nat) state"
 where
-    "number_list [] = pure []"
-  | "number_list (x # xs) = liftSt2 (op #) fresh (number_list xs)"
+    "number_list [] = pure_state []"
+  | "number_list (x # xs) = pure_state op # \<diamond> fresh \<diamond> number_list xs"
 
-lemma label_append: "number_list (a @ b) = liftSt2 (op @) (number_list a) (number_list b)"
+lemma number_list_append: "number_list (a @ b) = pure_state op @ \<diamond> number_list a \<diamond> number_list b"
 proof (induction a)
   case Nil
-  have "number_list b = liftSt2 (op @) (pure []) (number_list b)"
+  have "number_list b = pure_state op @ \<diamond> pure_state [] \<diamond> number_list b"
     by applicative_lifting simp
   thus ?case by simp
 next
   case (Cons a1 a2)
   let ?la2 = "number_list a2"
   let ?lb = "number_list b"
-  have "liftSt2 (op #) fresh (liftSt2 (op @) ?la2 ?lb) = liftSt2 (op @) (liftSt2 (op #) fresh ?la2) ?lb"
+  have "pure_state op # \<diamond> fresh \<diamond> (pure_state op @ \<diamond> ?la2 \<diamond> ?lb) =
+        pure_state op @ \<diamond> (pure_state op # \<diamond> fresh \<diamond> ?la2) \<diamond> ?lb"
     by applicative_lifting simp
   thus ?case using Cons.IH by simp
 qed
 
-lemma number_tree_list: "liftSt1 labels (number_tree t) = number_list (labels t)"
+lemma number_tree_list: "pure_state labels \<diamond> number_tree t = number_list (labels t)"
 proof (induction t)
   case (Leaf x)
-  have "liftSt1 labels (liftSt1 Leaf fresh) = liftSt2 (op #) fresh (Pair [])"
+  have "pure_state labels \<diamond> (pure_state Leaf \<diamond> fresh) = pure_state op # \<diamond> fresh \<diamond> pure_state []"
     by applicative_lifting simp
   thus ?case by simp
 next
   case (Node l r)
-  let ?ll = "liftSt1 labels (number_tree l)"
-  let ?lr = "liftSt1 labels (number_tree r)"
-  have "liftSt1 labels (liftSt2 Node (number_tree l) (number_tree r)) = liftSt2 (op @) ?ll ?lr"
+  let ?ll = "pure_state labels \<diamond> number_tree l"
+  let ?lr = "pure_state labels \<diamond> number_tree r"
+  have "pure_state labels \<diamond> (pure_state Node \<diamond> number_tree l \<diamond> number_tree r) =
+        pure_state op @ \<diamond> ?ll \<diamond> ?lr"
     by applicative_lifting simp
-  thus ?case using Node.IH by (simp add: label_append)
+  thus ?case using Node.IH by (simp add: number_list_append)
 qed
-
-experiment begin
-lemmas [simp] = liftSt1_def liftSt2_def
-
-lemma "Pair labels \<diamond> number_tree t = number_list (labels t)"
-proof (induction t)
-  case (Leaf x)
-  have "Pair labels \<diamond> (Pair Leaf \<diamond> fresh) = Pair op # \<diamond> fresh \<diamond> Pair []"
-    by applicative_lifting simp
-  thus ?case by simp
-next
-  case (Node l r)
-  let ?ll = "Pair labels \<diamond> number_tree l"
-  let ?lr = "Pair labels \<diamond> number_tree r"
-  have "Pair labels \<diamond> (Pair Node \<diamond> number_tree l \<diamond> number_tree r) = Pair op @ \<diamond> ?ll \<diamond> ?lr"
-    by applicative_lifting simp
-  thus ?case using Node.IH by (simp add: label_append)
-qed
-
-end
 
 end
